\addcontentsline{toc}{subsection}{Series \& Convergence}
\subsection*{Series \& Convergence}


\begin{tcolorbox}[title= DEFINITION OF CONVERGENT AND DIVERGENT SERIES,colframe=black,sharp corners,colback=white,colbacktitle=white,coltitle=black]

    For the infinite series $\displaystyle\sum_{n=1}^{\infty}a_n$, the \textbf{\textit{n}th partial sum} is given by
    \[S_n=a_1+a_2+a_3+...+a_n.\]
    If the sequence of partial sums $\{S_n\}$ converges to $S$, then the series $\displaystyle\sum_{n=1}^{\infty}a_n$ \textbf{converges}. The limit $S$ is called the \textbf{sum of the series}. 
    \[S_n=a_1+a_2+a_3+...+a_n \text{   where   }S=\sum_{n=1}^{\infty}a_n\]
    If $\{S_n\}$ diverges, then the series \textbf{diverges}.

\end{tcolorbox}
\vspace{.1in}

\noindent\textbf{Example: Convergent and Divergent Series}\\
Find the sequence of partial sums $S_1,\, S_2,\, S_3$ and an expression for $S_n$ for each of the following series. Determine its convergence or divergence.
\begin{parts}
    \part $\displaystyle\sum_{n=1}^{\infty}\frac{1}{2^n}=\frac{1}{2}+\frac{1}{4}+\frac{1}{8}+\frac{1}{16}+...$
    \vspace{\stretch{1}}
    
    \part $\displaystyle\sum_{n=1}^{\infty}\left(\frac{1}{n}-\frac{1}{n+1}\right)=\left(1-\frac{1}{2}\right)+\left(\frac{1}{2}-\frac{1}{3}\right)+\left(\frac{1}{3}-\frac{1}{4}\right)+...$
    \vspace{\stretch{1}}
    
    \part $\displaystyle\sum_{n=1}^{\infty}1=1+1+1+1+...$
    \vspace{\stretch{.2}}
\end{parts}


\noindent A \textbf{telescoping series} has the form $(b_1-b_2)+(b_2-b_3)+(b_3-b_4)+...$ therefore $S_n=b_1-b_{n+1}$. A telescoping series converges if and only if $b_n\rightarrow$ a finite number as $n\rightarrow\infty$. In which case, $\displaystyle S=b_1-\lim_{n\to\infty}b_{n+1}$.

\newpage


\noindent\textbf{Example: A Telescoping Series In Disguise}\\
Find the sum of the series $\displaystyle\sum_{n=1}^{\infty}\frac{2}{4n^2-1}$.
\vspace{\stretch{1}}


